simplify statements of lemmas in merkle and unreliable

theories/ub_logic/merkle/merkle_tree.v
@@ -216,7 +216,7 @@ Section merkle_tree.
   (*This lemma is here to ensure that the return value lies within a bound 
     This lemma is eventually used in the case where the proof is incorrect.
    *)
-  Lemma wp_compute_hash_from_leaf_size (n:nat) (tree:merkle_tree) (m:gmap nat Z) (v:nat) (proof:list (bool*nat)) lproof f E:
+  Local Lemma wp_compute_hash_from_leaf_size (n:nat) (tree:merkle_tree) (m:gmap nat Z) (v:nat) (proof:list (bool*nat)) lproof f E:
     {{{ ⌜tree_valid n tree m⌝ ∗
         coll_free_hashfun_amortized (val_size_for_hash)%nat max_hash_size f m ∗
         ⌜is_list proof lproof⌝ ∗
@@ -308,7 +308,7 @@ Section merkle_tree.
   Qed.
   
   (* The case where everything is correct *)
-  Lemma wp_compute_hash_from_leaf_correct (tree:merkle_tree) (m:gmap nat Z) (v:nat) (proof:list (bool*nat)) lproof f E:
+  Local Lemma wp_compute_hash_from_leaf_correct (tree:merkle_tree) (m:gmap nat Z) (v:nat) (proof:list (bool*nat)) lproof f E:
      {{{ ⌜tree_valid height tree m⌝ ∗
         coll_free_hashfun_amortized (val_size_for_hash)%nat max_hash_size f m ∗
         ⌜is_list proof lproof⌝ ∗
@@ -373,7 +373,7 @@ Section merkle_tree.
   Qed.
 
   (*The case where the leaf is incorrect*)
-  Lemma wp_compute_hash_from_leaf_incorrect (tree:merkle_tree) (m:gmap nat Z) (v v':nat) (proof:list (bool*nat)) lproof f E:
+  Local Lemma wp_compute_hash_from_leaf_incorrect (tree:merkle_tree) (m:gmap nat Z) (v v':nat) (proof:list (bool*nat)) lproof f E:
      {{{ ⌜tree_valid height tree m⌝ ∗
         coll_free_hashfun_amortized (val_size_for_hash)%nat max_hash_size f m ∗
         ⌜is_list proof lproof⌝ ∗
@@ -511,7 +511,7 @@ Section merkle_tree.
   Qed.
 
   (*The case where the leaf is correct but the proof is not *)
-  Lemma wp_compute_hash_from_leaf_incorrect_proof (tree:merkle_tree) (m:gmap nat Z) (v:nat) (proof:list (bool*nat)) lproof f E:
+  Local Lemma wp_compute_hash_from_leaf_incorrect_proof (tree:merkle_tree) (m:gmap nat Z) (v:nat) (proof:list (bool*nat)) lproof f E:
     {{{ ⌜tree_valid height tree m⌝ ∗
         coll_free_hashfun_amortized (val_size_for_hash)%nat max_hash_size f m ∗
         ⌜is_list proof lproof⌝ ∗
@@ -688,7 +688,17 @@ Section merkle_tree.
                 iPureIntro. by apply hash_bound_manipulation.
   Qed.
 
+  Definition is_possible_proof_list proof lproof tree :=
+    is_list proof lproof /\ possible_proof tree proof.
+
+  Definition tree_leaf_proof_match tree proof v :=
+    correct_proof tree proof /\ tree_leaf_value_match tree v proof.
+
   (** checker*)
+
+  Definition incorrect_proof_or_leaf tree proof v :=
+    incorrect_proof tree proof \/ (∃ v', tree_leaf_value_match tree v' proof /\ v ≠ v').
+  
   Definition merkle_tree_decider_program : val :=
     λ: "correct_root_hash" "lhmf",
       (λ: "lproof" "lleaf",
@@ -700,8 +710,7 @@ Section merkle_tree.
              {{{
                   ⌜tree_valid height tree m'⌝ ∗
                   coll_free_hashfun_amortized (val_size_for_hash)%nat max_hash_size f m' ∗
-                  ⌜is_list proof lproof⌝ ∗
-                  ⌜possible_proof tree proof ⌝∗
+                  ⌜is_possible_proof_list proof lproof tree ⌝∗
                   ⌜ size m' + (S height) <= max_hash_size⌝ ∗
                   € (nnreal_nat (S height) * amortized_error (val_size_for_hash)%nat max_hash_size max_hash_size_pos)%NNR
                    
@@ -709,13 +718,11 @@ Section merkle_tree.
               checker lproof (#v)
               {{{ (b:bool), RET #b;
                   if b then
-                    ⌜correct_proof tree proof⌝ ∗
-                    ⌜tree_leaf_value_match tree v proof⌝ ∗
+                    ⌜tree_leaf_proof_match tree proof v⌝∗
                     coll_free_hashfun_amortized (val_size_for_hash) max_hash_size f m' ∗
                     € (nnreal_nat (S height) * amortized_error (val_size_for_hash)%nat max_hash_size max_hash_size_pos)%NNR
                   else
-                    ⌜incorrect_proof tree proof \/
-                      (∃ v', tree_leaf_value_match tree v' proof /\ v ≠ v')⌝ ∗
+                    ⌜incorrect_proof_or_leaf tree proof v⌝ ∗
                     ∃ m'', ⌜m' ⊆ m''⌝ ∗
                         coll_free_hashfun_amortized (val_size_for_hash) max_hash_size f m'' ∗
                         ⌜size (m'') <= size m' + (S height)⌝ 
@@ -735,7 +742,7 @@ Section merkle_tree.
     rewrite /merkle_tree_decider_program.
     wp_pures. iModIntro.
     iApply "IH". iFrame.
-    iIntros (?????) "!> (%&H&%&%&%&Herr) HΦ".
+    iIntros (?????) "!> (%&H&[%%]&%&Herr) HΦ".
     wp_pures.
     epose proof (possible_proof_implies_exists_leaf tree proof _) as [v' ?].
     destruct (decide (v=v')).
@@ -757,7 +764,7 @@ Section merkle_tree.
           { intros K'; inversion K'; by subst. }
           iModIntro; iApply "HΦ".
           repeat iSplit.
-          -- iPureIntro. naive_solver.
+          -- iPureIntro. left. naive_solver.
           -- iExists _. by iFrame.
     - wp_apply (wp_compute_hash_from_leaf_incorrect with "[$H $Herr]").
       + repeat iSplit; done. 
@@ -816,10 +823,44 @@ Section merkle_tree.
     tree_leaf_list n b blist ->
     tree_leaf_list (S n) (Branch h a b) (alist ++ blist).
 
-  Lemma tree_leaf_list_length n tree lis:
-    tree_leaf_list n tree lis -> length lis = 2^n.
+  Definition tree_valid_with_leaf_list height tree list m:=
+    tree_leaf_list height tree list /\ tree_valid height tree m.
+
+  Lemma tree_valid_with_leaf_list_implies_tree_leaf_list h tree list m:
+    tree_valid_with_leaf_list h tree list m -> tree_leaf_list h tree list.
+  Proof.
+    by intros [].
+  Qed.
+
+  Lemma tree_valid_with_leaf_list_implies_tree_valid h tree list m:
+    tree_valid_with_leaf_list h tree list m -> tree_valid h tree m.
+  Proof.
+    by intros [].
+  Qed.
+
+  Lemma tree_valid_with_leaf_list_br h treea l1 (m:gmap nat Z) treeb l2 hash:
+    hash < 2 ^ val_bit_size ->
+    m !! (root_hash_value treea * 2 ^ val_bit_size + root_hash_value treeb) = Some (Z.of_nat hash)-> 
+    tree_valid_with_leaf_list h treea l1 m -> tree_valid_with_leaf_list h treeb l2 m ->
+    tree_valid_with_leaf_list (S h) (Branch hash treea treeb) (l1++l2) m.
   Proof.
     clear.
+    intros ? ?[??] [??]. split; by constructor.
+  Qed.
+  
+  Lemma tree_valid_with_leaf_list_superset m m' h tree l:
+    m⊆m' -> tree_valid_with_leaf_list h tree l m -> tree_valid_with_leaf_list h tree l m'.
+  Proof.
+    intros ? [??]. split; first done.
+    by eapply tree_valid_superset.
+  Qed.
+    
+
+  Lemma tree_valid_with_leaf_list_length n tree lis m:
+    tree_valid_with_leaf_list n tree lis m -> length lis = 2^n.
+  Proof.
+    clear.
+    intros [Hlist _]. revert Hlist.
     revert tree lis.
     induction n; intros tree lis Hlist.
     - inversion Hlist. by simpl.
@@ -827,15 +868,15 @@ Section merkle_tree.
       lia.
   Qed.
   
-  Lemma tree_leaf_list_implies_lookup_some lis tree h proof idx leafv:
-    tree_leaf_list h tree lis ->
+  Lemma tree_valid_with_leaf_list_implies_lookup_some lis tree h proof idx leafv m:
+    tree_valid_with_leaf_list h tree lis m ->
     proof_idx_relate h proof idx ->
     (tree_leaf_value_match tree leafv proof <->
     lis !! idx = Some leafv). 
   Proof.
     clear.
     revert lis tree proof idx leafv.
-    induction h as [|h IHheight]; intros lis tree proof idx leafv Hlist Hrelate.
+    induction h as [|h IHheight]; intros lis tree proof idx leafv [Hlist Hvalid] Hrelate.
     - split.
       + intros Hmatch. inversion Hrelate; inversion Hmatch; subst; try done.
         by inversion Hlist; subst.
@@ -844,25 +885,25 @@ Section merkle_tree.
         constructor.
     - split.
       + intros Hmatch. inversion Hrelate; subst.
-        * inversion Hrelate; inversion Hmatch; inversion Hlist; subst.
+        * inversion Hrelate; inversion Hmatch; inversion Hlist; inversion Hvalid; subst. inversion H15; inversion H22; subst.
           assert (length alist = 2^h).
-          { by eapply tree_leaf_list_length. }
+          { eapply tree_valid_with_leaf_list_length; split; try done. }
           rewrite lookup_app_l; last lia.
-          naive_solver.
-        * inversion Hrelate; inversion Hmatch; inversion Hlist; subst.
+          rewrite -IHheight; try done. 
+        * inversion Hrelate; inversion Hmatch; inversion Hlist; inversion Hvalid; subst. inversion H15; inversion H22; subst.
           assert (length alist = 2^h) as K.
-          { by eapply tree_leaf_list_length. }
+          { by eapply tree_valid_with_leaf_list_length. }
           rewrite lookup_app_r; last lia.
           rewrite K.
-          naive_solver.
+          by rewrite -IHheight.
       + intros Hfound.
-        pose proof (tree_leaf_list_length) as Hlen.
-        inversion Hrelate; inversion Hlist; subst.
-        * constructor.
+        pose proof (tree_valid_with_leaf_list_length) as Hlen.
+        inversion Hrelate; inversion Hlist; inversion Hvalid; subst.
+        * constructor. inversion H14; subst.
           rewrite IHheight; [|done|done].
           erewrite <-lookup_app_l; first done.
           by erewrite Hlen.
-        * constructor.
+        * constructor. inversion H14; subst.
           rewrite IHheight; [|done|done].
           erewrite <-Hlen; first erewrite <-lookup_app_r; try done.
           by erewrite Hlen.
